wip

Completeness.v
@@ -1,4 +1,4 @@
-From SymCoreTheory Require Import SymCore ConCore BranchLaws CostLaws.
+From SymCoreTheory Require Import SymCore ConCore CostLaws.
 From Stdlib Require Import Bool.Bool Arith.Wf_nat.
 From Stdlib Require Import Strings.String.
 From Stdlib Require Import Lists.List.
@@ -15,6 +15,7 @@ Definition target_completeness : Prop :=
     contains_env σ S Γs Γc ->
     contains σ S e_sym e_con ->
     concore_expr e_con ->
+    closed_program Γc e_con ->
     budget_total Φ Γs e_sym ->
     Γc ⊢ᶜ e_con ⇓ᶜ v_con ->
     exists h, forall n, (h <= n)%nat ->
@@ -28,6 +29,7 @@ Definition forall_form_lemma : Prop :=
       contains_env σ S Γs Γc ->
       contains σ S e_sym e_con ->
       concore_expr e_con ->
+      closed_program Γc e_con ->
       exists h, forall n, (h <= n)%nat ->
         forall v_sym, eval (Fin n) Φ Γs e_sym v_sym -> contains σ S v_sym v_con.
 
@@ -37,6 +39,7 @@ Definition existential_corollary : Prop :=
     contains_env σ S Γs Γc ->
     contains σ S e_sym e_con ->
     concore_expr e_con ->
+    closed_program Γc e_con ->
     budget_total Φ Γs e_sym ->
     Γc ⊢ᶜ e_con ⇓ᶜ v_con ->
     exists k v_sym, eval (Fin k) Φ Γs e_sym v_sym /\ contains σ S v_sym v_con.
@@ -44,8 +47,8 @@ Definition existential_corollary : Prop :=
 Lemma existential_corollary_of_target :
   target_completeness -> existential_corollary.
 Proof.
-  intros Htarget Φ Γs Γc σ S e_sym e_con v_con Hmod Henv Hcont Hcon Hbud Hevalc.
-  destruct (Htarget Φ Γs Γc σ S e_sym e_con v_con Hmod Henv Hcont Hcon Hbud Hevalc)
+  intros Htarget Φ Γs Γc σ S e_sym e_con v_con Hmod Henv Hcont Hcon Hcl Hbud Hevalc.
+  destruct (Htarget Φ Γs Γc σ S e_sym e_con v_con Hmod Henv Hcont Hcon Hcl Hbud Hevalc)
     as [h Hh].
   destruct (Hh h ltac:(lia)) as [v_sym [Heval Hcv]].
   exists h, v_sym. split; assumption.
@@ -594,7 +597,7 @@ Proof.
     assert (Hevinf : eval Inf Φ Γ (EApp ef ea) (reduce_prim p args'))
       by (eapply Eval_AppPrim; eassumption).
     split; [exact Hevinf |].
-    destruct (reduce_prim_contains_k σ S p ks args' (map ELit ls) HF) as [k' [Hk' Hc']].
+    destruct (reduce_prim_contains_k σ S p ks args' (map ELit ls) (closed_term_lits ls) HF) as [k' [Hk' Hc']].
     destruct (reduce_prim_literals_literal p ls) as [l0 Hl0]. rewrite Hl0 in Hc'.
     pose proof (smt_size_contains_k _ _ _ _ _ Hc') as Hsv. simpl in Hsv.
     rewrite prim_slack_literals in Hk'.
@@ -1656,10 +1659,11 @@ Qed.
 
 Lemma app_prim_core : forall Γc0 c1 c2 p args_c args_c' bk be,
   unspool_app (EApp c1 c2) [] = (EPrimOp p, args_c) ->
+  Forall closed_term args_c' ->
   Forall2 (fun a a' => good σ S (eq Γc0) a a') args_c args_c' ->
   core_at σ S (eq Γc0) (EApp c1 c2) (reduce_prim p args_c') bk be.
 Proof.
-  intros Γc0 c1 c2 p args_c args_c' bk be Hu HG.
+  intros Γc0 c1 c2 p args_c args_c' bk be Hu Hcl HG.
   destruct (args_good Γc0 args_c args_c' HG bk be) as [h0 [K0 H0]].
   exists (1 + h0), (K0 + prim_slack args_c').
   intros Γc Φ Γs e_s k kenv n v_s HA Hk Hkenv Hm Henv Hcont Hif Hn Hev. subst Γc.
@@ -1674,7 +1678,7 @@ Proof.
     destruct (H0 Φ Γs ks args_s a' kenv n ltac:(lia) Hkenv Hm Henv HF ltac:(lia) HE)
       as [ks' [HF' Hks']]
   end.
-  destruct (reduce_prim_contains_k σ S p ks' _ args_c' HF') as [k' [Hk' Hc']].
+  destruct (reduce_prim_contains_k σ S p ks' _ args_c' Hcl HF') as [k' [Hk' Hc']].
   exists k'. split; [lia | exact Hc'].
 Qed.
 
@@ -1829,108 +1833,145 @@ Context {sorts : SymCoreSorts} {solver : SymCoreSolver} {laws : SymFCCostLaws}.
 Context (σ : valuation) (S : symvars).
 
 Definition eval_motive (f : fuel) (Φ : path_condition) (Γ : environment) (e v : expr) : Prop :=
-  f = Inf -> Φ = pc_true -> concore_expr e -> concrete_env Γ -> good σ S (eq Γ) e v.
+  f = Inf -> Φ = pc_true -> concore_expr e -> concrete_env Γ -> closed_program Γ e ->
+  good σ S (eq Γ) e v.
 
 Definition fold_motive (f : fuel) (Φ : path_condition) (Γ : environment) (e : expr)
   (alts : list alt) (v : expr) : Prop :=
   f = Inf -> Φ = pc_true -> concore_expr e -> Forall concore_alt alts -> concrete_env Γ ->
+  scoped_env Γ -> closed_term e -> Forall (scoped_alt (dom_env Γ)) alts ->
   fgood σ S (eq Γ) e alts v.
 
 Lemma forall2_good_of_ind : forall Γ args args',
   Forall2 (fun a a' => eval Inf pc_true Γ a a' /\ eval_motive Inf pc_true Γ a a') args args' ->
-  Forall concore_expr args -> concrete_env Γ ->
+  Forall concore_expr args -> concrete_env Γ -> scoped_env Γ -> Forall (scoped (dom_env Γ)) args ->
   Forall2 (fun a a' => good σ S (eq Γ) a a') args args'.
 Proof.
-  intros Γ args args' HF Hc Hg. induction HF as [| a a' l l' [_ Ha] _ IH]; constructor.
-  - inversion Hc; subst. exact (Ha eq_refl eq_refl ltac:(assumption) Hg).
-  - inversion Hc; subst. exact (IH ltac:(assumption)).
+  intros Γ args args' HF Hc Hg HΓ Hs. induction HF as [| a a' l l' [_ Ha] _ IH]; constructor.
+  - inversion Hc; subst. inversion Hs; subst.
+    match goal with [Hca : concore_expr a, Hsa : scoped _ a |- _] =>
+      exact (Ha eq_refl eq_refl Hca Hg (conj HΓ Hsa)) end.
+  - inversion Hc; subst. inversion Hs; subst.
+    match goal with [Hcl : Forall concore_expr l, Hsl : Forall (scoped _) l |- _] =>
+      exact (IH Hcl Hsl) end.
+Qed.
+
+Lemma forall2_closed_of_ind : forall Γ args args',
+  Forall2 (fun a a' => eval Inf pc_true Γ a a' /\ eval_motive Inf pc_true Γ a a') args args' ->
+  Forall concore_expr args -> concrete_env Γ -> scoped_env Γ -> Forall (scoped (dom_env Γ)) args ->
+  Forall closed_term args'.
+Proof.
+  intros Γ args args' HF Hc Hg HΓ Hs. induction HF as [| a a' l l' [Hev _] _ IH]; constructor.
+  - inversion Hc; subst. inversion Hs; subst.
+    match goal with [Hca : concore_expr a, Hsa : scoped _ a |- _] =>
+      exact (closed_eval Γ a a' Hg Hca (conj HΓ Hsa) Hev) end.
+  - inversion Hc; subst. inversion Hs; subst.
+    match goal with [Hcl : Forall concore_expr l, Hsl : Forall (scoped _) l |- _] =>
+      exact (IH Hcl Hsl) end.
 Qed.
 
 Theorem concrete_good : forall Γc e_c v_c,
-  eval Inf pc_true Γc e_c v_c -> concore_expr e_c -> concrete_env Γc ->
+  eval Inf pc_true Γc e_c v_c -> concore_expr e_c -> concrete_env Γc -> closed_program Γc e_c ->
   good σ S (eq Γc) e_c v_c.
 Proof.
   intros Γc e_c v_c H.
   refine (eval_nested_ind eval_motive fold_motive _ _ _ _ _ _ _ _ _ _ _ _ _ _ _ _ _ _ _ _
             _ _ _ _ _ Inf pc_true Γc e_c v_c H eq_refl eq_refl);
     unfold eval_motive, fold_motive.
-  - intros f Φ Γ x Γ' e e' Hl _ IH Hf HΦ Hc Hg. injection Hf as ->. subst Φ.
+  - intros f Φ Γ x Γ' e e' Hl _ IH Hf HΦ Hc Hg Hcl. injection Hf as ->. subst Φ.
     destruct (lookup_env_concrete Γ x Γ' e Hg Hl) as [Hg' He].
+    destruct (lookup_env_scoped Γ x Γ' e (proj1 Hcl) Hl) as [HΓ' Hse].
     apply good_at_of_core. intros bk be _.
-    exact (var_core σ S Γ x Γ' e e' bk be Hl (IH eq_refl eq_refl He Hg')).
-  - intros f Φ Γ x Hl _ _ _ _. apply good_at_of_core. intros bk be _.
+    exact (var_core σ S Γ x Γ' e e' bk be Hl (IH eq_refl eq_refl He Hg' (conj HΓ' Hse))).
+  - intros f Φ Γ x Hl _ _ _ _ _. apply good_at_of_core. intros bk be _.
     exact (symvar_core σ S Γ x bk be Hl).
-  - intros f Φ Γ l _ _ _ _. apply good_at_of_core. intros bk be _. apply lit_core.
-  - intros f Φ Γ e d args Hu _ _ _ _. apply good_at_of_core. intros bk be _.
+  - intros f Φ Γ l _ _ _ _ _. apply good_at_of_core. intros bk be _. apply lit_core.
+  - intros f Φ Γ e d args Hu _ _ _ _ _. apply good_at_of_core. intros bk be _.
     exact (con_core σ S Γ e d args bk be Hu).
-  - intros f Φ Γ e γ e' _ IH Hf HΦ Hc Hg. injection Hf as ->. subst Φ.
+  - intros f Φ Γ e γ e' _ IH Hf HΦ Hc Hg Hcl. injection Hf as ->. subst Φ.
     apply good_at_of_core. intros bk be _.
-    exact (cast_core σ S Γ e γ e' bk be (IH eq_refl eq_refl (concore_expr_cast e γ Hc) Hg)).
-  - intros f Φ Γ Γ' x eb ea eb' _ IH Hf HΦ Hc Hg. injection Hf as ->. subst Φ.
+    exact (cast_core σ S Γ e γ e' bk be
+             (IH eq_refl eq_refl (concore_expr_cast e γ Hc) Hg (closed_program_cast _ _ _ Hcl))).
+  - intros f Φ Γ Γ' x eb ea eb' _ IH Hf HΦ Hc Hg Hcl. injection Hf as ->. subst Φ.
     pose proof (concore_expr_app_l _ _ Hc) as Hcf.
     pose proof (concore_expr_app_r _ _ Hc) as Hca.
     pose proof (concore_expr_lam _ _ (concore_expr_thunk _ _ Hcf)) as Hcb.
     pose proof (concore_expr_thunk_env _ _ Hcf) as Hg'.
     apply good_at_of_core. intros bk be _.
     exact (app_abs_core σ S Γ Γ' x eb ea eb'
-             (IH eq_refl eq_refl Hcb (concrete_env_extend Γ' x Γ ea Hg' Hg Hca)) Hca bk be).
-  - intros f Φ Γ ef ea ef' er Hcomp Hev1 IH1 _ IH2 Hf HΦ Hc Hg. injection Hf as ->. subst Φ.
+             (IH eq_refl eq_refl Hcb (concrete_env_extend Γ' x Γ ea Hg' Hg Hca)
+                (closed_program_abs _ _ _ _ _ Hcl)) Hca bk be).
+  - intros f Φ Γ ef ea ef' er Hcomp Hev1 IH1 _ IH2 Hf HΦ Hc Hg Hcl. injection Hf as ->. subst Φ.
     pose proof (concore_expr_app_l _ _ Hc) as Hcf.
     pose proof (concore_expr_app_r _ _ Hc) as Hca.
     pose proof (concore_eval_closed Γ ef ef' Hg Hcf Hev1) as Hcf'.
+    pose proof (closed_program_app_l _ _ _ Hcl) as Hclf.
+    pose proof (closed_eval Γ ef ef' Hg Hcf Hclf Hev1) as Hclf'.
+    assert (Hcl2 : closed_program Γ (EApp ef' ea)).
+    { split; [exact (proj1 Hcl) |].
+      apply Scoped_App; [exact (closed_term_scoped _ _ Hclf') | exact (proj2 (closed_program_app_r _ _ _ Hcl))]. }
     assert (Hl : forall l, spine_head ef <> ELit l).
     { intros l Hsh. pose proof (eval_spine_head_lit _ _ _ _ _ Hev1 eq_refl eq_refl l Hsh) as ->.
       inversion Hcomp. }
     apply good_at_of_core. intros bk be _.
-    exact (app_spine_core σ S Γ ef ea ef' er bk be Hcomp Hl (IH1 eq_refl eq_refl Hcf Hg)
-             (IH2 eq_refl eq_refl (Con_App _ _ Hcf' Hca) Hg)).
-  - intros f Φ Γ b _ _ _ _. apply good_at_of_core. intros bk be _. apply bot_core.
-  - intros f Φ Γ ef ea p args args' Hu _ HF Hf HΦ Hc Hg. injection Hf as ->. subst Φ.
+    exact (app_spine_core σ S Γ ef ea ef' er bk be Hcomp Hl (IH1 eq_refl eq_refl Hcf Hg Hclf)
+             (IH2 eq_refl eq_refl (Con_App _ _ Hcf' Hca) Hg Hcl2)).
+  - intros f Φ Γ b _ _ _ _ _. apply good_at_of_core. intros bk be _. apply bot_core.
+  - intros f Φ Γ ef ea p args args' Hu _ HF Hf HΦ Hc Hg Hcl. injection Hf as ->. subst Φ.
     destruct (unspool_app_concore _ _ _ _ Hu Hc (Forall_nil _)) as [_ Hargs].
+    destruct (unspool_app_scoped _ _ [] _ args Hu (proj2 Hcl) (Forall_nil _)) as [_ Hsargs].
     apply good_at_of_core. intros bk be _.
-    exact (app_prim_core σ S Γ ef ea p args args' bk be Hu (forall2_good_of_ind Γ args args' HF Hargs Hg)).
-  - intros f Φ Γ x e _ _ _ _. apply good_at_of_core. intros bk be _. apply lam_core.
-  - intros f Φ Γ ef γ ea γ_a γ_r er Hd _ IH Hf HΦ Hc Hg. injection Hf as ->. subst Φ.
+    exact (app_prim_core σ S Γ ef ea p args args' bk be Hu
+             (forall2_closed_of_ind Γ args args' HF Hargs Hg (proj1 Hcl) Hsargs)
+             (forall2_good_of_ind Γ args args' HF Hargs Hg (proj1 Hcl) Hsargs)).
+  - intros f Φ Γ x e _ _ _ _ _. apply good_at_of_core. intros bk be _. apply lam_core.
+  - intros f Φ Γ ef γ ea γ_a γ_r er Hd _ IH Hf HΦ Hc Hg Hcl. injection Hf as ->. subst Φ.
     pose proof (concore_expr_app_l _ _ Hc) as Hcf.
     pose proof (concore_expr_app_r _ _ Hc) as Hca.
     pose proof (concore_expr_cast _ _ Hcf) as Hcf0.
     apply good_at_of_core. intros bk be _.
     exact (app_cast_core σ S Γ ef γ ea γ_a γ_r er bk be Hd
-             (IH eq_refl eq_refl (Con_Cast _ _ (Con_App _ _ Hcf0 (Con_Cast _ _ Hca))) Hg)).
-  - intros f Φ Γ e1 e2 ec et ef args er Hu _ _ _ _ Hc _. exfalso.
+             (IH eq_refl eq_refl (Con_Cast _ _ (Con_App _ _ Hcf0 (Con_Cast _ _ Hca))) Hg
+                (closed_program_push _ _ _ _ _ _ Hcl))).
+  - intros f Φ Γ e1 e2 ec et ef args er Hu _ _ _ _ Hc _ _. exfalso.
     destruct (unspool_app_concore _ _ _ _ Hu Hc (Forall_nil _)) as [Hh _].
     exact (not_concore_if _ _ _ Hh).
-  - intros f Φ Γ b ea _ _ _ _. apply good_at_of_core. intros bk be _. apply app_bot_core.
-  - intros f Φ Γ es alts es' er Hev1 IH1 Hfold IHF Hf HΦ Hc Hg. injection Hf as ->. subst Φ.
+  - intros f Φ Γ b ea _ _ _ _ _. apply good_at_of_core. intros bk be _. apply app_bot_core.
+  - intros f Φ Γ es alts es' er Hev1 IH1 Hfold IHF Hf HΦ Hc Hg Hcl. injection Hf as ->. subst Φ.
     inversion Hc as [| | | | | | es0 alts0 Hces Halts | | | | | | |]; subst.
     pose proof (concore_eval_closed Γ es es' Hg Hces Hev1) as Hces'.
+    pose proof (closed_program_case_es _ _ _ Hcl) as Hcles.
+    pose proof (closed_eval Γ es es' Hg Hces Hcles Hev1) as Hcles'.
     change (dec Unlimited) with Inf in *.
     rewrite (merge_concore_id Γ es' Hces') in Hfold, IHF.
     apply good_at_of_core. intros bk be _.
-    exact (case_core σ S Γ es alts es' er bk be (IH1 eq_refl eq_refl Hces Hg)
-             (IHF eq_refl eq_refl Hces' Halts Hg) (fun Hi => fold_alts_inert _ _ _ _ _ _ Hi Hfold)).
+    exact (case_core σ S Γ es alts es' er bk be (IH1 eq_refl eq_refl Hces Hg Hcles)
+             (IHF eq_refl eq_refl Hces' Halts Hg (proj1 Hcl) Hcles' (closed_program_case_alts _ _ _ Hcl))
+             (fun Hi => fold_alts_inert _ _ _ _ _ _ Hi Hfold)).
   - intros. exfalso. match goal with [ Hc : concore_expr (EIf _ _ _) |- _ ] =>
       exact (not_concore_if _ _ _ Hc) end.
-  - intros f Φ Γ γ _ _ _ _. apply good_at_of_core. intros bk be _. apply coercion_core.
-  - intros f Φ Γ e Hs _ HΦ _ _. subst Φ. rewrite sat_pc_true in Hs. discriminate Hs.
-  - intros f Φ Γ τ _ _ _ _. apply good_at_of_core. intros bk be _. apply type_core.
-  - intros f Φ Γ Γ' e e' _ IH Hf HΦ Hc Hg. injection Hf as ->. subst Φ.
+  - intros f Φ Γ γ _ _ _ _ _. apply good_at_of_core. intros bk be _. apply coercion_core.
+  - intros f Φ Γ e Hs _ HΦ _ _ _. subst Φ. rewrite sat_pc_true in Hs. discriminate Hs.
+  - intros f Φ Γ τ _ _ _ _ _. apply good_at_of_core. intros bk be _. apply type_core.
+  - intros f Φ Γ Γ' e e' _ IH Hf HΦ Hc Hg Hcl. injection Hf as ->. subst Φ.
     apply (good_weaken σ S (fun _ => True)); [intros; exact I |].
     apply thunk_good.
-    exact (IH eq_refl eq_refl (concore_expr_thunk _ _ Hc) (concore_expr_thunk_env _ _ Hc)).
+    exact (IH eq_refl eq_refl (concore_expr_thunk _ _ Hc) (concore_expr_thunk_env _ _ Hc)
+             (closed_program_thunk _ _ _ Hcl)).
   - intros Φ Γ e Hf. discriminate Hf.
   - intros. exfalso. match goal with [ Hc : concore_expr (EIf _ _ _) |- _ ] =>
       exact (not_concore_if _ _ _ Hc) end.
   - intros. exfalso. match goal with [ Hc : concore_expr (EIf _ _ _) |- _ ] =>
       exact (not_concore_if _ _ _ Hc) end.
-  - intros f Φ Γ e d ea xs ep alts er Hd Hfa _ IH Hf HΦ Hc Halts Hg. subst f Φ.
+  - intros f Φ Γ e d ea xs ep alts er Hd Hfa _ IH Hf HΦ Hc Halts Hg HΓ Hcle Hsalts. subst f Φ.
     pose proof (decompose_con_app_concore e d ea Hd Hc) as Hea.
     pose proof (find_alt_concore d alts xs ep Hfa Halts) as Hep.
     apply fgood_of_core. intros bk be _.
     exact (fcon_core σ S Γ e d ea xs ep alts er bk be Hd Hfa Hea
-             (IH eq_refl eq_refl Hep (concrete_env_extend_multi xs ea Γ Γ Hg Hg Hea))).
-  - intros f Φ Γ b alts _ _ _ _ _. apply fgood_of_core. intros bk be _. apply fbot_core.
-  - intros f Φ Γ e alts _ Hmatch Hbot _ _ _ _ _. apply fgood_of_core. intros bk be _.
+             (IH eq_refl eq_refl Hep (concrete_env_extend_multi xs ea Γ Γ Hg Hg Hea)
+                (closed_program_fold_con Γ e d ea alts xs ep HΓ Hcle Hsalts Hd Hfa))).
+  - intros f Φ Γ b alts _ _ _ _ _ _ _ _. apply fgood_of_core. intros bk be _. apply fbot_core.
+  - intros f Φ Γ e alts _ Hmatch Hbot _ _ _ _ _ _ _ _. apply fgood_of_core. intros bk be _.
     exact (fotherwise_core σ S Γ e alts bk be Hmatch Hbot).
 Qed.
 
@@ -1941,13 +1982,14 @@ Theorem forall_form : forall Γc e_con v_con,
     contains_env σ S Γs Γc ->
     contains σ S e_sym e_con ->
     concore_expr e_con ->
+    closed_program Γc e_con ->
     exists h, forall n, (h <= n)%nat ->
       forall v_sym, eval (Fin n) Φ Γs e_sym v_sym -> contains σ S v_sym v_con.
 Proof.
-  intros Γc e_con v_con Hevc Φ Γs e_sym Hm Henv Hcont Hcon.
+  intros Γc e_con v_con Hevc Φ Γs e_sym Hm Henv Hcont Hcon Hcl.
   destruct (contains_k_of_contains _ _ _ _ Hcont) as [k Hk].
   destruct (contains_env_k_of_contains_env _ _ _ _ Henv) as [kenv Hkenv].
-  destruct (concrete_good Γc e_con v_con Hevc Hcon (contains_env_concrete σ S Γs Γc Henv)
+  destruct (concrete_good Γc e_con v_con Hevc Hcon (contains_env_concrete σ S Γs Γc Henv) Hcl
               (k + kenv) (k + kenv)) as [h [K H]].
   exists h. intros n Hn v_sym Hv.
   destruct (H Γc Φ Γs e_sym k kenv n v_sym eq_refl ltac:(lia) ltac:(lia) Hm Hkenv Hk Hn Hv)
@@ -1962,14 +2004,14 @@ Context {sorts : SymCoreSorts} {solver : SymCoreSolver} {laws : SymFCCostLaws}.
 
 Theorem concore_completeness_forall : forall_form_lemma.
 Proof.
-  intros Γc e_con v_con Hevc Φ Γs σ S e_sym Hm Henv Hcont Hcon.
-  exact (forall_form σ S Γc e_con v_con Hevc Φ Γs e_sym Hm Henv Hcont Hcon).
+  intros Γc e_con v_con Hevc Φ Γs σ S e_sym Hm Henv Hcont Hcon Hcl.
+  exact (forall_form σ S Γc e_con v_con Hevc Φ Γs e_sym Hm Henv Hcont Hcon Hcl).
 Qed.
 
 Theorem concore_completeness_budget : target_completeness.
 Proof.
-  intros Φ Γs Γc σ S e_sym e_con v_con Hm Henv Hcont Hcon [hb Hb] Hevc.
-  destruct (forall_form σ S Γc e_con v_con Hevc Φ Γs e_sym Hm Henv Hcont Hcon) as [h Hh].
+  intros Φ Γs Γc σ S e_sym e_con v_con Hm Henv Hcont Hcon Hcl [hb Hb] Hevc.
+  destruct (forall_form σ S Γc e_con v_con Hevc Φ Γs e_sym Hm Henv Hcont Hcon Hcl) as [h Hh].
   exists (h + hb). intros n Hn.
   destruct (Hb n ltac:(lia)) as [v Hv].
   exists v. split; [exact Hv | exact (Hh n ltac:(lia) v Hv)].
